Stateful HMAC-SHA2_256: enforcing the same val declarations for the bundle module

code/experimental/hmac/HMAC_SHA2_256.fst
@@ -1,105 +1,73 @@
 module HMAC_SHA2_256
 
 open FStar.Mul
+open FStar.Ghost
 open FStar.HyperStack
 open FStar.ST
 open FStar.Buffer
+
+open C.Loops
+
+open Hacl.Cast
+open Hacl.UInt8
+open Hacl.UInt32
 open FStar.UInt32
 
-module Buffer = FStar.Buffer
-module MAC    = Hacl.HMAC.SHA2.L256
+
+(* Definition of aliases for modules *)
+module U8 = FStar.UInt8
+module U32 = FStar.UInt32
+module U64 = FStar.UInt64
+
+module H8 = Hacl.UInt8
+module H32 = Hacl.UInt32
+module H64 = Hacl.UInt64
+
+module Spec_Hash = Spec.SHA2_256
+module Hash = Hacl.Hash.SHA2_256
+module Spec = Spec.HMAC.SHA2_256
+module MAC = Hacl.HMAC.SHA2_256
 
 
 (* Definition of base types *)
-let uint8_t   = FStar.UInt8.t
-let uint32_t  = FStar.UInt32.t
-let uint64_t  = FStar.UInt64.t
+private let uint8_t   = FStar.UInt8.t
+private let uint32_t  = FStar.UInt32.t
+private let uint64_t  = FStar.UInt64.t
 
-let suint8_t  = Hacl.UInt8.t
-let suint32_t = Hacl.UInt32.t
-let suint64_t = Hacl.UInt64.t
+private let uint8_ht  = Hacl.UInt8.t
+private let uint32_ht = Hacl.UInt32.t
+private let uint64_ht = Hacl.UInt64.t
 
-let suint32_p = Buffer.buffer suint32_t
-let suint8_p  = Buffer.buffer suint8_t
-
+private let uint32_p = Buffer.buffer uint32_ht
+private let uint8_p  = Buffer.buffer uint8_ht
 
 
 //
-// HMAC
+// HMAC-SHA2_256
 //
 
-inline_for_extraction let hmac_hashsize_256 = MAC.size_hash
-inline_for_extraction let hmac_blocksize_256 = MAC.size_block
-inline_for_extraction let hmac_size_state_256 = MAC.size_state
-
-
-val hmac_sha2_init_256:
-  state :suint32_p{length state = v hmac_size_state_256} ->
-  key   :suint8_p ->
-  len   :uint32_t {v len = length key} ->
+val hmac_core:
+  mac  :uint8_p  {length mac = v Hash.size_hash} ->
+  key  :uint8_p  {length key = v Hash.size_block /\ disjoint key mac} ->
+  data :uint8_p  {length data + v Hash.size_block < Spec_Hash.max_input_len_8 /\ disjoint data mac /\ disjoint data key} ->
+  len  :uint32_t {length data = v len} ->
   Stack unit
-        (requires (fun h0 -> live h0 state /\ live h0 key))
-        (ensures  (fun h0 r h1 -> live h1 state /\ modifies_1 state h0 h1))
+        (requires (fun h -> live h mac /\ live h key /\ live h data))
+        (ensures  (fun h0 _ h1 -> live h1 mac /\ modifies_1 mac h0 h1))
 
-let hmac_sha2_init_256 state key len = MAC.init state key len
+let hmac_core mac key data len = MAC.hmac_core mac key data len
 
+//
+//
 
-
-val hmac_sha2_update_256 :
-  state :suint32_p{length state = v hmac_size_state_256} ->
-  data  :suint8_p {length data = v hmac_blocksize_256} ->
+val hmac:
+  mac     :uint8_p  {length mac = v Hash.size_hash} ->
+  key     :uint8_p  {length key = v Hash.size_block /\ disjoint key mac} ->
+  keylen  :uint32_t {v keylen = length key} ->
+  data    :uint8_p  {length data + v Hash.size_block < Spec_Hash.max_input_len_8 /\ disjoint data mac /\ disjoint data key} ->
+  datalen :uint32_t {v datalen = length data} ->
   Stack unit
-        (requires (fun h0 -> live h0 state /\ live h0 data))
-        (ensures  (fun h0 r h1 -> live h1 state /\ modifies_1 state h0 h1))
+        (requires (fun h -> live h mac /\ live h key /\ live h data))
+        (ensures  (fun h0 _ h1 -> live h1 mac /\ modifies_1 mac h0 h1))
 
-let hmac_sha2_update_256 state data = MAC.update state data
-
-
-
-val hmac_sha2_update_multi_256:
-  state :suint32_p{length state = v hmac_size_state_256} ->
-  data  :suint8_p ->
-  n     :uint32_t{v n * v hmac_blocksize_256 <= length data} ->
-  idx   :uint32_t{v idx <= v n} ->
-  Stack unit
-        (requires (fun h0 -> live h0 state /\ live h0 data))
-        (ensures  (fun h0 _ h1 -> live h1 state /\ modifies_1 state h0 h1))
-
-let hmac_sha2_update_multi_256 state data n idx = MAC.update_multi state data n idx
-
-
-
-val hmac_sha2_update_last_256:
-  state :suint32_p{length state = v hmac_size_state_256} ->
-  data  :suint8_p {length data <= v hmac_blocksize_256} ->
-  len   :uint32_t {v len = length data} ->
-  Stack unit
-        (requires (fun h0 -> live h0 state /\ live h0 data))
-        (ensures  (fun h0 r h1 -> live h1 state /\ modifies_1 state h0 h1))
-
-let hmac_sha2_update_last_256 state data len = MAC.update_last state data len
-
-
-
-val hmac_sha2_finish_256:
-  state :suint32_p{length state = v hmac_size_state_256} ->
-  mac   :suint8_p {length mac = v hmac_hashsize_256} ->
-  Stack unit
-        (requires (fun h0 -> live h0 state /\ live h0 mac))
-        (ensures  (fun h0 _ h1 -> live h1 state /\ live h1 mac /\ modifies_2 state mac h0 h1))
-
-let hmac_sha2_finish_256 state mac = MAC.finish state mac
-
-
-
-val hmac_sha2_256:
-  mac     :suint8_p{length mac = v hmac_hashsize_256} ->
-  key     :suint8_p ->
-  keylen  :uint32_t{v keylen = length key} ->
-  data    :suint8_p ->
-  datalen :uint32_t{v datalen = length data /\ v datalen + v hmac_blocksize_256 <= pow2 32} ->
-  Stack unit
-        (requires (fun h -> live h mac /\ live h key /\ live h data ))
-        (ensures  (fun h0 r h1 -> live h1 mac /\ modifies_1 mac h0 h1))
-
-let hmac_sha2_256 mac key keylen data datalen = MAC.hmac mac key keylen data datalen
+let hmac mac key keylen data datalen = MAC.hmac mac key keylen data datalen
